Diff/ResourceExhaustion.v
@@ -1,0 +1,178 @@
+Require Import ClassicalExtras.
+
+Require Import TraceModel.
+Require Import Properties.
+Require Import Galois.
+
+Set Bullet Behavior "Strict Subproofs".
+
+(* This file is intentionaly NOT included in _CoqProject *)
+
+
+Axiom event : Set.
+Axiom is_event : Events event.
+Hint Resolve is_event.
+
+Axiom endstate : Set.
+Axiom is_endstate : EndState endstate.
+Hint Resolve is_endstate.
+
+Definition endstateS : Set := endstate.
+Lemma is_endstateS : EndState endstateS.
+Proof.
+  trivial.
+Qed.
+
+Definition out_of_memory := unit.
+Definition endstateT : Set := endstate + out_of_memory.
+Definition OOM : endstateT := inr tt.
+Hint Unfold endstateT OOM.
+Lemma is_endstateT : EndState endstateT.
+Proof.
+  now repeat constructor.
+Qed.
+
+Definition traceS := trace event endstateS.
+Definition traceT := trace event endstateT.
+Definition finprefS := finpref event endstateS.
+Definition finprefT := finpref event endstateT.
+
+Definition propS := prop event endstateS.
+Definition propT := prop event endstateT.
+Definition fpropS := fprop event endstateS.
+Definition fpropT := fprop event endstateT.
+
+Inductive syntactic_eq : traceS -> traceT -> Prop :=
+| syntactic_eq_tstop : forall l es,
+    syntactic_eq (tstop l es) (tstop l (inl es))
+| syntactic_eq_tsilent : forall l,
+    syntactic_eq (tsilent _ l) (tsilent _ l)
+| syntactic_eq_tstream : forall s,
+    syntactic_eq (tstream _ s) (tstream _ s)
+.
+Notation "t__s '≡' t__t" := (syntactic_eq t__s t__t) (no associativity, at level 10).
+Hint Constructors syntactic_eq.
+
+Axiom prefixTS : finprefT -> traceS -> Prop.
+
+Definition rel : traceS -> traceT -> Prop :=
+  fun t__s t__t => t__s ≡ t__t \/ exists m, (t__t = tstop m OOM /\ prefixTS (ftbd _ m) t__s).
+Hint Unfold rel.
+
+Inductive syntactic_eq_finpref : finprefS -> finprefT -> Prop :=
+| syntactic_eq_fstop : forall l es,
+    syntactic_eq_finpref (fstop l es) (fstop l (inl es))
+| syntactic_eq_ftbd : forall l,
+    syntactic_eq_finpref (ftbd _ l) (ftbd _ l)
+.
+
+Definition rel_finpref : finprefS -> finprefT -> Prop :=
+  fun m__s m__t => syntactic_eq_finpref m__s m__t \/ exists l, (m__t = fstop l OOM /\ prefix_finpref (ftbd _ l) m__s).
+
+Definition GC_traceT_traceS : Galois_Connection traceT traceS :=
+  induced_connection rel.
+
+Definition τ : propS -> propT := α GC_traceT_traceS.
+Definition σ : propT -> propS := γ GC_traceT_traceS.
+
+Lemma τ_preserves_dense : forall (π : propS),
+    Dense π -> Dense (τ π).
+Proof.
+  unfold Dense, τ, GC_traceT_traceS, induced_connection, low_rel; simpl.
+  intros π HDense.
+  intros t__t Hfin.
+  destruct t__t as [l [e | []] | l | s].
+  - exists (tstop l e). split.
+    apply HDense. econstructor; eexists; eauto.
+    left; eauto.
+  - exists (tstop l (an_endstate is_endstateS)). split.
+    apply HDense. econstructor; eexists; eauto.
+    right; eexists; split; eauto.
+    admit. (* property of prefixTS *)
+  - destruct Hfin as [l' [e' Hn]].
+    inversion Hn.
+  - destruct Hfin as [l' [e' Hn]].
+    inversion Hn.
+Admitted.
+
+Lemma σ_preserves_dense : forall (π : propT),
+    Dense π -> Dense (σ π).
+Proof.
+  unfold Dense, σ, GC_traceT_traceS, induced_connection, up_rel; simpl.
+  intros π HDense.
+  intros t__s Hfin t__t Hrel.
+  destruct Hrel as [Hrel | Hrel].
+  - apply HDense; inversion Hrel; subst.
+    + now repeat eexists.
+    + destruct Hfin as [l' [e' Hn]].
+      inversion Hn.
+    + destruct Hfin as [l' [e' Hn]].
+      inversion Hn.
+  - destruct Hrel as [m [Heq Hpref]].
+    apply HDense.
+    rewrite Heq.
+    now repeat eexists.
+Qed.
+
+
+(* The goal is now to prove that τ and/or σ preserve Safety. 
+   I need to define σ and τ for fprop, in order to use them
+   to transform the set of bad prefixes *)
+
+Definition traceT_to_traceS_safety (t__t : traceT) : traceS :=
+  match t__t with
+  | tstop l (inl e) => tstop l e
+  | tstop l (inr _) => tstop l (an_endstate is_endstateS)
+  | tsilent l => tsilent _ l
+  | tstream s => tstream _ s
+  end.
+Hint Unfold traceT_to_traceS_safety.
+
+Lemma traceT_to_traceS_safety_rel : forall (t__t : traceT),
+    rel (traceT_to_traceS_safety t__t) t__t.
+Proof.
+  intros t__t.
+  destruct t__t as [l [e | []] | l | s]; try now repeat constructor.
+  - right.
+    exists l. split. reflexivity.
+    admit. (* trivial property of prefixTS *)
+Admitted.
+
+Definition finprefT_to_finprefS (m__t : finprefT) : finprefS :=
+  match m__t with
+  | fstop l (inl e) => fstop l e
+  | fstop l (inr _) => ftbd _ l
+  | ftbd l => ftbd _ l
+  end.
+
+(* Lemma prefix_T_to_S_safety : forall (m__t : finprefT) (t__t : traceT), *)
+(*    prefix (finprefT_to_finprefT_safety m__t) (traceT_to_traceS_safety t__t) -> *)
+(*    prefix m__t t__t. *)
+(* Proof. *)
+(*   intros m__t t__t Hpref. *)
+(*   destruct m__t as [l [e | []] | l]; *)
+(*     destruct t__t as [l' [e' | []] | l' | s']; *)
+(*     try now auto. *)
+(*   - destruct Hpref; split; now subst. *)
+(*   - simpl in Hpref. *)
+
+Definition traceS_to_traceT (t__s : traceS) : traceT :=
+  match t__s with
+  | tstop l e => tstop l (inl e)
+  | tsilent l => tsilent _ l
+  | tstream s => tstream _ s
+  end.
+Hint Unfold traceS_to_traceT.
+
+Lemma traceS_to_traceT_rel : forall (t__s : traceS),
+    rel t__s (traceS_to_traceT t__s).
+Proof.
+  intros t__s.
+  destruct t__s; now repeat constructor.
+Qed.
+
+Definition finprefS_to_finprefT (m__s : finprefS) : finprefT :=
+  match m__s with
+  | fstop l e => fstop l (inl e)
+  | ftbd l => ftbd _ l
+  end.
